policies/PVI.v
@@ -48,7 +48,7 @@ Module PVI <: Policy.
   
   Definition CallT (l:loc) (pct pt: tag) : PolicyResult tag := PolicySuccess pct.
 
-  Definition ArgT (l:loc) (pct vt : tag) (f x: ident) : PolicyResult (tag * tag) := PolicySuccess (pct,vt).
+  Definition ArgT (l:loc) (pct fpt vt : tag) (idx:nat) (ty: type) : PolicyResult (tag * tag) := PolicySuccess (pct,vt).
 
   Definition RetT (l:loc) (pct_clr pct_cle vt : tag) : PolicyResult (tag * tag) := PolicySuccess (pct_cle,vt).
   
